Kraken/X64/Sep.lean
@@ -11,12 +11,12 @@ theorem store_sep (s : MachineData) (addr : BitVec 64) (w : Width) (v : w.type) 
     (bs : List UInt8) (R : DataMem → Prop)
     (h_mem : s.dmem =⋆ Eq (bs.At addr) ⋆ R)
     (h_len : bs.length = w.bytes) :
-    have mem' := Mem.storeInt s.dmem addr w.bytes v.toInt
+    have mem' := Mem.storeBV s.dmem addr w.bytes v
     MachineData.store s addr v ret =
       require_write_access addr w (fun _ =>
         ret { s with dmem := mem' }) := by
-  have h_load : Mem.loadInt s.dmem addr w.bytes = some (Int.ofBytes bs) :=
-    Mem.loadInt_sep bs addr w.bytes R s.dmem h_mem h_len (by cases w <;> decide)
+  have h_load : Mem.loadBytes s.dmem addr w.bytes = some bs :=
+    Mem.loadBytes_sep bs addr w.bytes R s.dmem h_mem h_len (by cases w <;> decide)
   simp only [MachineData.store, h_load]
 
 @[kspec]
@@ -25,6 +25,6 @@ theorem load_sep (s : MachineData) (addr : BitVec 64) (w : Width) (ret : w.type 
     (h_mem : s.dmem =⋆ Eq (bs.At addr) ⋆ R)
     (h_len : bs.length = w.bytes) :
     MachineData.load s addr w ret =
-      require_read_access addr w (fun _ => ret (.ofInt w.bits (Int.ofBytes bs)) s) := by
+      require_read_access addr w (fun _ => ret (BitVec.ofBytes w.bits bs) s) := by
   simp only [MachineData.load,
-    Mem.loadInt_sep bs addr w.bytes R s.dmem h_mem h_len (by cases w <;> decide)]
+    Mem.loadBV_sep bs addr w.bits w.bytes R s.dmem h_mem h_len (by cases w <;> decide)]
